codelib/CodeLib/SepLogic/WasmRules.lean
@@ -566,7 +566,7 @@ theorem Mem.write32_eq_self {m : Mem} {addr value : UInt32}
       bv_decide
     · rfl
 
-theorem store32Heap_pointsTo [WasmHeapGS]
+theorem store32Heap_pointsTo {α : Type} [WasmHeapGS α]
     (σ : WasmHeapMap (Option UInt8)) (memId : Nat) (addr value : UInt32)
     (h0 : get? σ ⟨memId, addr⟩ = none)
     (h1 : get? σ ⟨memId, addr + 1⟩ = none)
@@ -576,11 +576,11 @@ theorem store32Heap_pointsTo [WasmHeapGS]
     (_hn2 : (addr + 2).toNat = addr.toNat + 2)
     (_hn3 : (addr + 3).toNat = addr.toNat + 3) :
     ([∗map] address ↦ byte ∈ store32Heap σ memId addr value,
-      pointsTo (GF := WasmHeapGF) (H := WasmHeapMap)
+      pointsTo (GF := WasmHeapGF.{0} α) (H := WasmHeapMap)
         address (DFrac.own 1) byte) ⊢
       pointsTo_u32 memId addr value ∗
       ([∗map] address ↦ byte ∈ σ,
-        pointsTo (GF := WasmHeapGF) (H := WasmHeapMap)
+        pointsTo (GF := WasmHeapGF.{0} α) (H := WasmHeapMap)
           address (DFrac.own 1) byte) := by
   have h01 : (⟨memId, addr + 1⟩ : MemoryKey) ≠ ⟨memId, addr⟩ := fun h =>
     absurd (congrArg MemoryKey.addr h) (by intro h'; simp at h')
@@ -730,7 +730,7 @@ def store64Heap (σ : WasmHeapMap (Option UInt8)) (memId : Nat) (addr : UInt32)
       ⟨memId, addr + 6⟩ (some (u64Byte value 6)))
     ⟨memId, addr + 7⟩ (some (u64Byte value 7))
 
-theorem store64Heap_pointsTo [WasmHeapGS]
+theorem store64Heap_pointsTo {α : Type} [WasmHeapGS α]
     (σ : WasmHeapMap (Option UInt8)) (memId : Nat) (addr : UInt32) (value : UInt64)
     (h0 : get? σ ⟨memId, addr⟩ = none)
     (h1 : get? (insert σ ⟨memId, addr⟩ (some (u64Byte value 0))) ⟨memId, addr + 1⟩ = none)
@@ -783,11 +783,11 @@ theorem store64Heap_pointsTo [WasmHeapGS]
           ⟨memId, addr + 5⟩ (some (u64Byte value 5)))
         ⟨memId, addr + 6⟩ (some (u64Byte value 6))) ⟨memId, addr + 7⟩ = none) :
     ([∗map] address ↦ byte ∈ store64Heap σ memId addr value,
-      pointsTo (GF := WasmHeapGF) (H := WasmHeapMap)
+      pointsTo (GF := WasmHeapGF.{0} α) (H := WasmHeapMap)
         address (DFrac.own 1) byte) ⊢
       pointsTo_u64 memId addr value ∗
       ([∗map] address ↦ byte ∈ σ,
-        pointsTo (GF := WasmHeapGF) (H := WasmHeapMap)
+        pointsTo (GF := WasmHeapGF.{0} α) (H := WasmHeapMap)
           address (DFrac.own 1) byte) := by
   unfold store64Heap
   rw [(BI.BigSepM.bigSepM_insert h7).to_eq]
